improve compose macro and renamings

LeanSubst/Basic.lean
@@ -1,18 +1,12 @@
 import Lilac
--- TODO:
--- Generalizing to vector substitutions is a matter of the following change:
--- `SubstMap S T` becomes `SubstMap n S (T n)` for `T : Nat -> Type`
--- would want to make sure that length 1 substitutions are still nice to work with
-
--- Scoped versus Unscoped, does not appear to be a natural way to generalize to have
--- one development that gives both, easiest method would be to maintain two copies
--- Scoped is the natural consequence of `Ren n m := Fin n -> Fin m`
 
 namespace LeanSubst
   universe u
   variable {S T : Type}
 
   def Ren := Sequ Nat
+
+  def Ren.id : Ren := λ x => x
 
   def Ren.lift (r : Ren) (k : Nat := 1) : Ren
   | n => if n < k then n else r (n - k) + k
@@ -86,7 +80,7 @@ namespace LeanSubst
 
   @[simp, grind =]
   theorem Ren.to_id : Ren.to (T := T) id = +0 := by
-    unfold Ren.to; unfold Subst.id; simp
+    unfold Ren.to; unfold Subst.id; simp [id]
 
   @[simp, grind =]
   theorem Ren.to_succ : Ren.to (T := T) (· + 1) = +1 := by
@@ -105,13 +99,21 @@ namespace LeanSubst
   theorem Ren.lift_zero {r : Ren} : r.lift 0 = r := by
     unfold Ren.lift; funext; case _ i => grind
 
-  @[simp, grind =]
+  @[grind =]
   theorem Ren.lift_succ {r : Ren} {k} : r.lift (k + 1) = (r.lift k).lift := by
     induction k; simp
     case _ n ih =>
       unfold Ren.lift; funext; case _ i =>
       simp; unfold Ren.lift at ih; simp at ih
       grind
+
+  @[simp]
+  theorem Red.id_action {x} : Ren.id x = x := by simp [Ren.id]
+
+  @[simp]
+  theorem Ren.lift_id : Ren.lift Ren.id = Ren.id := by
+    funext; case _ x =>
+    cases x <;> simp [lift, id]
 
   @[grind =]
   theorem Ren.to_lift [RenMap T] {r : Ren} {k} : (r.lift k).to = (@Ren.to T r).lift k := by
@@ -136,10 +138,17 @@ namespace LeanSubst
     funext; case _ x =>
     cases x <;> simp [Ren.to, Subst.compose]
 
+  macro:max t:term noWs "⟨" r:term "⟩" : term => `(rmap $r $t)
   macro:max t:term noWs "[" σ:term "]" : term => `(smap1 $σ $t)
   macro:max t:term noWs "[" σ:term ":" T:term "]" : term => `(smap (T := $T) $σ $t)
+  infixr:85 " ∘ " => Ren.compose
   infixr:85 " ∘ " => Subst.compose
   infixr:85 " ◾ " => Subst.hcompose
+
+  @[app_unexpander rmap]
+  def unexpandRenApply : Lean.PrettyPrinter.Unexpander
+  | `($_ $r $t) => `($t⟨$r⟩)
+  | _ => throw ()
 
   @[app_unexpander smap1]
   def unexpandSubstApply1 : Lean.PrettyPrinter.Unexpander
@@ -151,5 +160,52 @@ namespace LeanSubst
   | `($_ $σ $t) => `($t[$σ : _])
   | `($_ (T := $T) $σ $t) => `($t[$σ : $T])
   | _ => throw ()
+
+  instance : HAndThen Ren Ren Ren where
+    hAndThen f g := (g ()) ∘ f
+
+  instance : HAndThen (Nat -> Nat) Ren Ren where
+    hAndThen f g := (g ()) ∘ f
+
+  instance : HAndThen Ren (Nat -> Nat) Ren where
+    hAndThen f g := (g ()) ∘ f
+
+  instance : HAndThen (Sequ Nat) Ren Ren where
+    hAndThen f g := (g ()) ∘ f
+
+  instance : HAndThen Ren (Sequ Nat) Ren where
+    hAndThen f g := (g ()) ∘ f
+
+  @[simp]
+  theorem Ren.id_promote : (λ x => x) = id := by unfold Ren.id; simp
+
+  @[simp]
+  theorem Ren.post_compose_id_left {r : Ren} : id >> r = r := by
+    simp [HAndThen.hAndThen]; unfold id; unfold Function.comp; simp
+
+  @[simp]
+  theorem Ren.post_compose_id_right {r : Ren} : r >> id = r := by
+    simp [HAndThen.hAndThen]; unfold id; unfold Function.comp; simp
+
+  @[simp]
+  theorem Ren.post_compose_assoc {r1 r2 r3 : Ren} : (r1 >> r2) >> r3 = r1 >> r2 >> r3 := by
+    simp [HAndThen.hAndThen]; unfold Function.comp; simp
+
+  @[simp]
+  theorem Ren.post_compose_action {r1 r2 : Ren} {x} : (r1 >> r2) x = r2 (r1 x) := by
+    simp [HAndThen.hAndThen]
+
+  theorem Ren.post_compose_lift_k1 {r1 r2 : Ren} : (r1 >> r2).lift = r1.lift >> r2.lift := by
+    funext; case _ x =>
+    cases x <;> simp [Ren.lift]
+
+  @[simp]
+  theorem Ren.post_compose_lift {k} {r1 r2 : Ren} : (r1 >> r2).lift k = r1.lift k >> r2.lift k := by
+    induction k generalizing r1 r2; simp
+    case _ k ih =>
+      rw [lift_succ, ih]
+      rw [lift_succ (r := r1)]
+      rw [lift_succ (r := r2)]
+      rw [post_compose_lift_k1]
 
 end LeanSubst
